<?xml version="1.0"?>
<rdf:RDF xmlns="https://w3id.org/OPLa/"
     xml:base="https://w3id.org/OPLa/"
     xmlns:dc="http://purl.org/dc/elements/1.1/"
     xmlns:owl="http://www.w3.org/2002/07/owl#"
     xmlns:rdf="http://www.w3.org/1999/02/22-rdf-syntax-ns#"
     xmlns:xml="http://www.w3.org/XML/1998/namespace"
     xmlns:xsd="http://www.w3.org/2001/XMLSchema#"
     xmlns:opla="https://w3id.org/OPLa/"
     xmlns:rdfs="http://www.w3.org/2000/01/rdf-schema#">
    <owl:Ontology rdf:about="https://w3id.org/OPLa/">
        <dc:creator>Aldo Gangemi</dc:creator>
        <dc:creator>Cogan Shimizu</dc:creator>
        <dc:creator>Karl Hammar</dc:creator>
        <dc:creator>Luigi Asprino</dc:creator>
        <dc:creator>Pascal Hitzler</dc:creator>
        <dc:creator>Valentina Carriero</dc:creator>
        <dc:creator>Valentina Presutti</dc:creator>
        <rdfs:comment xml:lang="en">This is the OPLa ontology, a simple representation language for ontollgy design patterns. Central to this language is the use of OWL annotation properties. Such annotation properties are used to indicate ontology design patterns and to represent relationships between patterns and ontology modules, as well as to indicate how patterns can be related to their more abstract counterparts (knowledge patterns/conceptual components) and to RDF graphs including triples that comply with them.</rdfs:comment>
        <rdfs:label xml:lang="en">OPLa (Ontology Pattern Language)</rdfs:label>
        <owl:versionInfo>0.0.1</owl:versionInfo>
    </owl:Ontology>
    


    <!-- 
    ///////////////////////////////////////////////////////////////////////////////////////
    //
    // Annotation properties
    //
    ///////////////////////////////////////////////////////////////////////////////////////
     -->

    


    <!-- http://purl.org/dc/elements/1.1/creator -->

    <owl:AnnotationProperty rdf:about="http://purl.org/dc/elements/1.1/creator"/>
    


    <!-- https://w3id.org/OPLa/addressesScenario -->

    <owl:AnnotationProperty rdf:about="https://w3id.org/OPLa/addressesScenario">
        <rdfs:comment xml:lang="en">This property relates an Ontological Collection to examples of instantiation of the Ontological Collection.</rdfs:comment>
        <rdfs:label xml:lang="en">addresses scenario</rdfs:label>
        <rdfs:range rdf:resource="http://www.w3.org/2001/XMLSchema#string"/>
        <rdfs:domain rdf:resource="https://w3id.org/OPLa/OntologicalCollection"/>
    </owl:AnnotationProperty>
    


    <!-- https://w3id.org/OPLa/compliesWith -->

    <owl:AnnotationProperty rdf:about="https://w3id.org/OPLa/compliesWith">
        <rdfs:comment xml:lang="en">This property relates an RDF graph to the implemented pattern it complies with.</rdfs:comment>
        <rdfs:label xml:lang="en">complies with</rdfs:label>
        <rdfs:range rdf:resource="https://w3id.org/OPLa/ImplementedPattern"/>
        <rdfs:domain rdf:resource="https://w3id.org/OPLa/RDFGraph"/>
    </owl:AnnotationProperty>
    


    <!-- https://w3id.org/OPLa/componentOfPattern -->

    <owl:AnnotationProperty rdf:about="https://w3id.org/OPLa/componentOfPattern">
        <rdfs:comment xml:lang="en">This property relates a Pattern to the Pattern it is a component of.</rdfs:comment>
        <rdfs:label xml:lang="en">component of pattern</rdfs:label>
        <rdfs:subPropertyOf rdf:resource="https://w3id.org/OPLa/hasRelatedPattern"/>
        <rdfs:range rdf:resource="https://w3id.org/OPLa/ImplementedPattern"/>
        <rdfs:domain rdf:resource="https://w3id.org/OPLa/ImplementedPattern"/>
    </owl:AnnotationProperty>
    


    <!-- https://w3id.org/OPLa/coversRequirement -->

    <owl:AnnotationProperty rdf:about="https://w3id.org/OPLa/coversRequirement">
        <rdfs:comment xml:lang="en">This property relates an Ontological Collection to possible requirements (e.g. in the form of competency questions) the Ontological Collection provides a solution for.</rdfs:comment>
        <rdfs:label xml:lang="en">covers requirement</rdfs:label>
        <rdfs:range rdf:resource="http://www.w3.org/2001/XMLSchema#string"/>
        <rdfs:domain rdf:resource="https://w3id.org/OPLa/OntologicalCollection"/>
    </owl:AnnotationProperty>
    


    <!-- https://w3id.org/OPLa/derivedFromModule -->

    <owl:AnnotationProperty rdf:about="https://w3id.org/OPLa/derivedFromModule">
        <rdfs:comment xml:lang="en">This property relates a Module to the Module it is a derived from.</rdfs:comment>
        <rdfs:label xml:lang="en">derived from module</rdfs:label>
        <rdfs:subPropertyOf rdf:resource="https://w3id.org/OPLa/hasRelatedModule"/>
        <rdfs:range rdf:resource="https://w3id.org/OPLa/Module"/>
        <rdfs:domain rdf:resource="https://w3id.org/OPLa/Module"/>
    </owl:AnnotationProperty>
    


    <!-- https://w3id.org/OPLa/derivedFromPattern -->

    <owl:AnnotationProperty rdf:about="https://w3id.org/OPLa/derivedFromPattern">
        <rdfs:comment xml:lang="en">This property relates a Pattern to the Pattern it is a derived from.</rdfs:comment>
        <rdfs:label xml:lang="en">derived from pattern</rdfs:label>
        <rdfs:subPropertyOf rdf:resource="https://w3id.org/OPLa/hasRelatedPattern"/>
        <rdfs:range rdf:resource="https://w3id.org/OPLa/ImplementedPattern"/>
        <rdfs:domain rdf:resource="https://w3id.org/OPLa/ImplementedPattern"/>
    </owl:AnnotationProperty>
    


    <!-- https://w3id.org/OPLa/description -->

    <owl:AnnotationProperty rdf:about="https://w3id.org/OPLa/description">
        <rdfs:comment xml:lang="en">This property relates anything to its description.</rdfs:comment>
        <rdfs:label xml:lang="en">description</rdfs:label>
        <rdfs:range rdf:resource="http://www.w3.org/2001/XMLSchema#string"/>
        <rdfs:domain rdf:resource="http://www.w3.org/2002/07/owl#Thing"/>
    </owl:AnnotationProperty>
    


    <!-- https://w3id.org/OPLa/entityPosition -->

    <owl:AnnotationProperty rdf:about="https://w3id.org/OPLa/entityPosition">
        <rdfs:comment xml:lang="en">This property has a blank node as its target. This blank node is intended to &quot;encapsulate&quot; all other position related annotations.</rdfs:comment>
        <rdfs:label xml:lang="en">entity position</rdfs:label>
        <rdfs:range rdf:resource="http://www.w3.org/2002/07/owl#Thing"/>
        <rdfs:domain rdf:resource="https://w3id.org/OPLa/Class"/>
    </owl:AnnotationProperty>
    


    <!-- https://w3id.org/OPLa/entityPositionX -->

    <owl:AnnotationProperty rdf:about="https://w3id.org/OPLa/entityPositionX">
        <rdfs:comment xml:lang="en">This property specifies the X coordinate (expressed as a double) of a node in a schema diagram.</rdfs:comment>
        <rdfs:label xml:lang="en">entity position X</rdfs:label>
        <rdfs:range rdf:resource="http://www.w3.org/2000/01/rdf-schema#Literal"/>
        <rdfs:domain rdf:resource="http://www.w3.org/2002/07/owl#Thing"/>
    </owl:AnnotationProperty>
    


    <!-- https://w3id.org/OPLa/entityPositionY -->

    <owl:AnnotationProperty rdf:about="https://w3id.org/OPLa/entityPositionY">
        <rdfs:comment xml:lang="en">This property specifies the Y coordinate (expressed as a double) of a node in a schema diagram.</rdfs:comment>
        <rdfs:label xml:lang="en">entity position Y</rdfs:label>
        <rdfs:range rdf:resource="http://www.w3.org/2000/01/rdf-schema#Literal"/>
        <rdfs:domain rdf:resource="http://www.w3.org/2002/07/owl#Thing"/>
    </owl:AnnotationProperty>
    


    <!-- https://w3id.org/OPLa/extractedFrom -->

    <owl:AnnotationProperty rdf:about="https://w3id.org/OPLa/extractedFrom">
        <rdfs:comment xml:lang="en">This property relates an Ontological Collection to a possible reference ontology which the annotated Ontological Collection was extracted from (i.e. the reference ontology that the ontology elements have been deeply or partially cloned by).</rdfs:comment>
        <rdfs:label xml:lang="en">extracted from</rdfs:label>
        <rdfs:range rdf:resource="https://w3id.org/OPLa/OntologicalCollection"/>
        <rdfs:domain rdf:resource="https://w3id.org/OPLa/OntologicalCollection"/>
    </owl:AnnotationProperty>
    


    <!-- https://w3id.org/OPLa/generalizationOfConceptualComponent -->

    <owl:AnnotationProperty rdf:about="https://w3id.org/OPLa/generalizationOfConceptualComponent">
        <rdfs:comment xml:lang="en">This property relates a Conceptual Component to the Conceptual Component it is a generalization of.</rdfs:comment>
        <rdfs:label xml:lang="en">generalization of conceptual component</rdfs:label>
        <rdfs:subPropertyOf rdf:resource="https://w3id.org/OPLa/hasRelatedConceptualComponent"/>
        <rdfs:range rdf:resource="https://w3id.org/OPLa/ConceptualComponent"/>
        <rdfs:domain rdf:resource="https://w3id.org/OPLa/ConceptualComponent"/>
    </owl:AnnotationProperty>
    


    <!-- https://w3id.org/OPLa/generalizationOfModule -->

    <owl:AnnotationProperty rdf:about="https://w3id.org/OPLa/generalizationOfModule">
        <rdfs:comment xml:lang="en">This property relates a Module to the Module it is a generalization of.</rdfs:comment>
        <rdfs:label xml:lang="en">generalization of module</rdfs:label>
        <rdfs:subPropertyOf rdf:resource="https://w3id.org/OPLa/hasRelatedModule"/>
        <rdfs:range rdf:resource="https://w3id.org/OPLa/Module"/>
        <rdfs:domain rdf:resource="https://w3id.org/OPLa/Module"/>
    </owl:AnnotationProperty>
    


    <!-- https://w3id.org/OPLa/generalizationOfPattern -->

    <owl:AnnotationProperty rdf:about="https://w3id.org/OPLa/generalizationOfPattern">
        <rdfs:comment xml:lang="en">This property relates a Pattern to the Pattern it is a generalization of.</rdfs:comment>
        <rdfs:label xml:lang="en">generalization of pattern</rdfs:label>
        <rdfs:subPropertyOf rdf:resource="https://w3id.org/OPLa/hasRelatedPattern"/>
        <rdfs:range rdf:resource="https://w3id.org/OPLa/ImplementedPattern"/>
        <rdfs:domain rdf:resource="https://w3id.org/OPLa/ImplementedPattern"/>
    </owl:AnnotationProperty>
    


    <!-- https://w3id.org/OPLa/hasCompetencyQuestion -->

    <owl:AnnotationProperty rdf:about="https://w3id.org/OPLa/hasCompetencyQuestion">
        <rdfs:comment xml:lang="en">This property relates an Ontological Collection, an Ontology Design Pattern or a Conceptual Component to an addressed Competency Question (expressed in natural language) that can be evaluated against them.</rdfs:comment>
        <rdfs:label xml:lang="en">has competency question</rdfs:label>
        <rdfs:range rdf:resource="http://www.w3.org/2001/XMLSchema#string"/>
        <rdfs:domain rdf:resource="http://www.w3.org/2002/07/owl#Thing"/>
    </owl:AnnotationProperty>
    


    <!-- https://w3id.org/OPLa/hasConsequence -->

    <owl:AnnotationProperty rdf:about="https://w3id.org/OPLa/hasConsequence">
        <rdfs:comment xml:lang="en">This property relates an Ontological Collection to the description of the benefits and/or possible trade-offs when using the Ontological Collection.</rdfs:comment>
        <rdfs:label xml:lang="en">has consequence</rdfs:label>
        <rdfs:range rdf:resource="http://www.w3.org/2001/XMLSchema#string"/>
        <rdfs:domain rdf:resource="https://w3id.org/OPLa/OntologicalCollection"/>
    </owl:AnnotationProperty>
    


    <!-- https://w3id.org/OPLa/hasDomain -->

    <owl:AnnotationProperty rdf:about="https://w3id.org/OPLa/hasDomain">
        <rdfs:comment xml:lang="en">This property relates an entity to its domain (e.g. multimedia, time).</rdfs:comment>
        <rdfs:label xml:lang="en">has domain</rdfs:label>
        <rdfs:range rdf:resource="https://w3id.org/OPLa/Domain"/>
        <rdfs:domain rdf:resource="http://www.w3.org/2002/07/owl#Thing"/>
    </owl:AnnotationProperty>
    


    <!-- https://w3id.org/OPLa/hasIntent -->

    <owl:AnnotationProperty rdf:about="https://w3id.org/OPLa/hasIntent">
        <rdfs:comment xml:lang="en">This property relates an Ontological Collection to its intent.</rdfs:comment>
        <rdfs:label xml:lang="en">has intent</rdfs:label>
        <rdfs:range rdf:resource="http://www.w3.org/2001/XMLSchema#string"/>
        <rdfs:domain rdf:resource="https://w3id.org/OPLa/OntologicalCollection"/>
    </owl:AnnotationProperty>
    


    <!-- https://w3id.org/OPLa/hasRelatedConceptualComponent -->

    <owl:AnnotationProperty rdf:about="https://w3id.org/OPLa/hasRelatedConceptualComponent">
        <rdfs:comment xml:lang="en">This property relates a Conceptual Component to another Conceptual Component.</rdfs:comment>
        <rdfs:label xml:lang="en">has related conceptual component</rdfs:label>
        <rdfs:range rdf:resource="https://w3id.org/OPLa/ConceptualComponent"/>
        <rdfs:domain rdf:resource="https://w3id.org/OPLa/ConceptualComponent"/>
    </owl:AnnotationProperty>
    


    <!-- https://w3id.org/OPLa/hasRelatedModule -->

    <owl:AnnotationProperty rdf:about="https://w3id.org/OPLa/hasRelatedModule">
        <rdfs:comment xml:lang="en">This property relates a Module to another Module. It does not need to be derived from a module, they simply share the same intent.</rdfs:comment>
        <rdfs:label xml:lang="en">has related module</rdfs:label>
        <rdfs:range rdf:resource="https://w3id.org/OPLa/Module"/>
        <rdfs:domain rdf:resource="https://w3id.org/OPLa/Module"/>
    </owl:AnnotationProperty>
    


    <!-- https://w3id.org/OPLa/hasRelatedPattern -->

    <owl:AnnotationProperty rdf:about="https://w3id.org/OPLa/hasRelatedPattern">
        <rdfs:comment xml:lang="en">This property relates a Pattern to another Pattern. It does not need to be derived from a pattern, they simply share the same intent.</rdfs:comment>
        <rdfs:label xml:lang="en">has related pattern</rdfs:label>
        <rdfs:range rdf:resource="https://w3id.org/OPLa/ImplementedPattern"/>
        <rdfs:domain rdf:resource="https://w3id.org/OPLa/ImplementedPattern"/>
    </owl:AnnotationProperty>
    


    <!-- https://w3id.org/OPLa/hasUnitTest -->

    <owl:AnnotationProperty rdf:about="https://w3id.org/OPLa/hasUnitTest">
        <rdfs:comment xml:lang="en">This property relates an Ontological Collection to a unit test (e.g. in the form of a SPARQL query) to be launched to evaluate the ontological collection against a requirement-based task.</rdfs:comment>
        <rdfs:label xml:lang="en">has unit test</rdfs:label>
        <rdfs:range rdf:resource="http://www.w3.org/2001/XMLSchema#string"/>
        <rdfs:domain rdf:resource="https://w3id.org/OPLa/OntologicalCollection"/>
    </owl:AnnotationProperty>
    


    <!-- https://w3id.org/OPLa/implementsConceptualComponent -->

    <owl:AnnotationProperty rdf:about="https://w3id.org/OPLa/implementsConceptualComponent">
        <rdfs:comment xml:lang="en">This property relates a Module to the Conceptual Component it implements.</rdfs:comment>
        <rdfs:label xml:lang="en">implements conceptual component</rdfs:label>
        <rdfs:range rdf:resource="https://w3id.org/OPLa/ConceptualComponent"/>
        <rdfs:domain rdf:resource="https://w3id.org/OPLa/Module"/>
    </owl:AnnotationProperty>
    


    <!-- https://w3id.org/OPLa/implementsOntologyDesignPattern -->

    <owl:AnnotationProperty rdf:about="https://w3id.org/OPLa/implementsOntologyDesignPattern">
        <rdfs:comment xml:lang="en">This property relates an implemented pattern to the ontology design pattern it implements, i.e. providing a conceptual model expressed in an OWL file to an ontology design pattern intended as a template.</rdfs:comment>
        <rdfs:label xml:lang="en">implements ontology design pattern</rdfs:label>
        <rdfs:range rdf:resource="https://w3id.org/OPLa/OntologyDesignPattern"/>
        <rdfs:domain rdf:resource="https://w3id.org/OPLa/ImplementedPattern"/>
    </owl:AnnotationProperty>
    


    <!-- https://w3id.org/OPLa/includesImplementedPattern -->

    <owl:AnnotationProperty rdf:about="https://w3id.org/OPLa/includesImplementedPattern">
        <rdfs:comment xml:lang="en">This property relates a module to an implemented pattern it includes.</rdfs:comment>
        <rdfs:label xml:lang="en">includes implemented pattern</rdfs:label>
        <rdfs:range rdf:resource="https://w3id.org/OPLa/ImplementedPattern"/>
        <rdfs:domain rdf:resource="https://w3id.org/OPLa/Module"/>
    </owl:AnnotationProperty>
    


    <!-- https://w3id.org/OPLa/includesModule -->

    <owl:AnnotationProperty rdf:about="https://w3id.org/OPLa/includesModule">
        <rdfs:comment xml:lang="en">This property relates an ontology to a module, intended as an ontology fragment, it includes.</rdfs:comment>
        <rdfs:label xml:lang="en">includes module</rdfs:label>
        <rdfs:range rdf:resource="https://w3id.org/OPLa/Module"/>
        <rdfs:domain rdf:resource="https://w3id.org/OPLa/Ontology"/>
    </owl:AnnotationProperty>
    


    <!-- https://w3id.org/OPLa/isMemberOf -->

    <owl:AnnotationProperty rdf:about="https://w3id.org/OPLa/isMemberOf">
        <rdfs:comment xml:lang="en">This property relates an RDF statement or a single node to the RDF graph reification it is member of.</rdfs:comment>
        <rdfs:label xml:lang="en">is member of</rdfs:label>
        <rdfs:range rdf:resource="https://w3id.org/OPLa/RDFGraph"/>
        <rdfs:domain rdf:resource="https://w3id.org/OPLa/OntologicalEntity"/>
    </owl:AnnotationProperty>
    


    <!-- https://w3id.org/OPLa/isNativeTo -->

    <owl:AnnotationProperty rdf:about="https://w3id.org/OPLa/isNativeTo">
        <rdfs:comment xml:lang="en">This property relates an Ontological Entity to an Ontological Collection it is native to, i.e. which is a core element of.</rdfs:comment>
        <rdfs:label xml:lang="en">is native to</rdfs:label>
        <rdfs:range rdf:resource="https://w3id.org/OPLa/OntologicalCollection"/>
        <rdfs:domain rdf:resource="https://w3id.org/OPLa/OntologicalEntity"/>
    </owl:AnnotationProperty>
    


    <!-- https://w3id.org/OPLa/modelFor -->

    <owl:AnnotationProperty rdf:about="https://w3id.org/OPLa/modelFor">
        <rdfs:comment xml:lang="en">This property relates an ontology design pattern to the conceptual component it provides a model for.</rdfs:comment>
        <rdfs:label xml:lang="en">model for</rdfs:label>
        <rdfs:range rdf:resource="https://w3id.org/OPLa/ConceptualComponent"/>
        <rdfs:domain rdf:resource="https://w3id.org/OPLa/OntologyDesignPattern"/>
    </owl:AnnotationProperty>
    


    <!-- https://w3id.org/OPLa/name -->

    <owl:AnnotationProperty rdf:about="https://w3id.org/OPLa/name">
        <rdfs:comment xml:lang="en">This property relates anything to its name.</rdfs:comment>
        <rdfs:label xml:lang="en">name</rdfs:label>
        <rdfs:range rdf:resource="http://www.w3.org/2001/XMLSchema#string"/>
        <rdfs:domain rdf:resource="http://www.w3.org/2002/07/owl#Thing"/>
    </owl:AnnotationProperty>
    


    <!-- https://w3id.org/OPLa/ofExternalType -->

    <owl:AnnotationProperty rdf:about="https://w3id.org/OPLa/ofExternalType">
        <rdfs:comment xml:lang="en">This property indicates that another pattern may hook into this entity. For example, a hook might indicate that the pattern developer acknowledges a certain concept is out of scope of the particular pattern.</rdfs:comment>
        <rdfs:label xml:lang="en">of external type</rdfs:label>
    </owl:AnnotationProperty>
    


    <!-- https://w3id.org/OPLa/provides -->

    <owl:AnnotationProperty rdf:about="https://w3id.org/OPLa/provides">
        <rdfs:comment xml:lang="en">This property relates an ontology design pattern to the interface it provides, i.e. when it formally specificies a concept used in the interface, which can be referred to by another ontology design pattern.</rdfs:comment>
        <rdfs:label xml:lang="en">provides</rdfs:label>
        <rdfs:range rdf:resource="https://w3id.org/OPLa/Interface"/>
        <rdfs:domain rdf:resource="https://w3id.org/OPLa/OntologyDesignPattern"/>
    </owl:AnnotationProperty>
    


    <!-- https://w3id.org/OPLa/reengineeredFrom -->

    <owl:AnnotationProperty rdf:about="https://w3id.org/OPLa/reengineeredFrom">
        <rdfs:comment xml:lang="en">This property relates an Ontological Collection to a concept schema, page, or anything else from which the annotated Ontological Collection was reengineered. If the source does not have any URI e.g., a printed book, this property value should provide information as precise as possible in order to identify the source. This property is alternative to the extractedFrom property because it is used when the pattern come from a concept schema which is not an owl ontology.</rdfs:comment>
        <rdfs:label xml:lang="en">reengineered from</rdfs:label>
        <rdfs:range rdf:resource="http://www.w3.org/2002/07/owl#Thing"/>
        <rdfs:domain rdf:resource="https://w3id.org/OPLa/OntologicalCollection"/>
    </owl:AnnotationProperty>
    


    <!-- https://w3id.org/OPLa/requires -->

    <owl:AnnotationProperty rdf:about="https://w3id.org/OPLa/requires">
        <rdfs:comment xml:lang="en">This property relates an ontology design pattern to the interface it requires, i.e. when it referes to an external concept not formally specified in the ODP.</rdfs:comment>
        <rdfs:label xml:lang="en">requires</rdfs:label>
        <rdfs:range rdf:resource="https://w3id.org/OPLa/Interface"/>
        <rdfs:domain rdf:resource="https://w3id.org/OPLa/OntologyDesignPattern"/>
    </owl:AnnotationProperty>
    


    <!-- https://w3id.org/OPLa/reusesAsTemplate -->

    <owl:AnnotationProperty rdf:about="https://w3id.org/OPLa/reusesAsTemplate">
        <rdfs:comment xml:lang="en">This property relates an Ontological Collection to another Ontological Collection that is reused as template.</rdfs:comment>
        <rdfs:label xml:lang="en">reuses as template</rdfs:label>
        <rdfs:range rdf:resource="https://w3id.org/OPLa/OntologicalCollection"/>
        <rdfs:domain rdf:resource="https://w3id.org/OPLa/OntologicalCollection"/>
    </owl:AnnotationProperty>
    


    <!-- https://w3id.org/OPLa/specializationOfConceptualComponent -->

    <owl:AnnotationProperty rdf:about="https://w3id.org/OPLa/specializationOfConceptualComponent">
        <rdfs:comment xml:lang="en">This property relates a Conceptual Component to the Conceptual Component it is a specialization of.</rdfs:comment>
        <rdfs:label xml:lang="en">specialization of conceptual component</rdfs:label>
        <rdfs:subPropertyOf rdf:resource="https://w3id.org/OPLa/hasRelatedConceptualComponent"/>
        <rdfs:range rdf:resource="https://w3id.org/OPLa/ConceptualComponent"/>
        <rdfs:domain rdf:resource="https://w3id.org/OPLa/ConceptualComponent"/>
    </owl:AnnotationProperty>
    


    <!-- https://w3id.org/OPLa/specializationOfModule -->

    <owl:AnnotationProperty rdf:about="https://w3id.org/OPLa/specializationOfModule">
        <rdfs:comment xml:lang="en">This property relates a Module to the Module it is a specialization of.</rdfs:comment>
        <rdfs:label xml:lang="en">specialization of module</rdfs:label>
        <rdfs:subPropertyOf rdf:resource="https://w3id.org/OPLa/hasRelatedModule"/>
        <rdfs:range rdf:resource="https://w3id.org/OPLa/Module"/>
        <rdfs:domain rdf:resource="https://w3id.org/OPLa/Module"/>
    </owl:AnnotationProperty>
    


    <!-- https://w3id.org/OPLa/specializationOfPattern -->

    <owl:AnnotationProperty rdf:about="https://w3id.org/OPLa/specializationOfPattern">
        <rdfs:comment xml:lang="en">This property relates a Pattern to the Pattern it is a specialization of.</rdfs:comment>
        <rdfs:label xml:lang="en">specialization of pattern</rdfs:label>
        <rdfs:subPropertyOf rdf:resource="https://w3id.org/OPLa/hasRelatedPattern"/>
        <rdfs:range rdf:resource="https://w3id.org/OPLa/ImplementedPattern"/>
        <rdfs:domain rdf:resource="https://w3id.org/OPLa/ImplementedPattern"/>
    </owl:AnnotationProperty>
    


    <!-- 
    ///////////////////////////////////////////////////////////////////////////////////////
    //
    // Classes
    //
    ///////////////////////////////////////////////////////////////////////////////////////
     -->

    


    <!-- https://w3id.org/OPLa/Axiom -->

    <owl:Class rdf:about="https://w3id.org/OPLa/Axiom">
        <rdfs:subClassOf rdf:resource="https://w3id.org/OPLa/OntologicalEntity"/>
        <rdfs:comment xml:lang="en">This class represents an axiom.</rdfs:comment>
        <rdfs:label xml:lang="en">Axiom</rdfs:label>
    </owl:Class>
    


    <!-- https://w3id.org/OPLa/Class -->

    <owl:Class rdf:about="https://w3id.org/OPLa/Class">
        <rdfs:subClassOf rdf:resource="https://w3id.org/OPLa/OntologicalEntity"/>
        <rdfs:comment xml:lang="en">This class represents a class.</rdfs:comment>
        <rdfs:label xml:lang="en">Class</rdfs:label>
    </owl:Class>
    


    <!-- https://w3id.org/OPLa/ConceptualComponent -->

    <owl:Class rdf:about="https://w3id.org/OPLa/ConceptualComponent">
        <rdfs:comment xml:lang="en">A conceptual component is the most abstract notion of pattern, one that is shared as the cognitive structure for organising our knowledge about a specific modelling issue.</rdfs:comment>
        <rdfs:label xml:lang="en">Conceptual Component</rdfs:label>
        <rdfs:label xml:lang="en">Knowledge Pattern</rdfs:label>
    </owl:Class>
    


    <!-- https://w3id.org/OPLa/Domain -->

    <owl:Class rdf:about="https://w3id.org/OPLa/Domain">
        <rdfs:comment xml:lang="en">This class represents a domain, an area of interest.</rdfs:comment>
        <rdfs:label xml:lang="en">Domain</rdfs:label>
    </owl:Class>
    


    <!-- https://w3id.org/OPLa/ImplementedPattern -->

    <owl:Class rdf:about="https://w3id.org/OPLa/ImplementedPattern">
        <rdfs:subClassOf rdf:resource="https://w3id.org/OPLa/OntologicalCollection"/>
        <rdfs:comment xml:lang="en">An implemented pattern is an OWL implementation of an ontology design pattern in a defined namespace.</rdfs:comment>
        <rdfs:label xml:lang="en">Implemented Pattern</rdfs:label>
        <rdfs:label xml:lang="en">Pattern Instance</rdfs:label>
    </owl:Class>
    


    <!-- https://w3id.org/OPLa/Individual -->

    <owl:Class rdf:about="https://w3id.org/OPLa/Individual">
        <rdfs:subClassOf rdf:resource="https://w3id.org/OPLa/OntologicalEntity"/>
        <rdfs:comment xml:lang="en">This class represents an individual.</rdfs:comment>
        <rdfs:label xml:lang="en">Individual</rdfs:label>
    </owl:Class>
    


    <!-- https://w3id.org/OPLa/Interface -->

    <owl:Class rdf:about="https://w3id.org/OPLa/Interface">
        <rdfs:comment xml:lang="en">An Interface is a placeholder e.g. in an ontology design pattern, which only identifies key concepts, and can be implemented by different ontology design patterns.</rdfs:comment>
        <rdfs:label xml:lang="en">Interface</rdfs:label>
    </owl:Class>
    


    <!-- https://w3id.org/OPLa/Module -->

    <owl:Class rdf:about="https://w3id.org/OPLa/Module">
        <rdfs:subClassOf rdf:resource="https://w3id.org/OPLa/OntologicalCollection"/>
        <rdfs:comment xml:lang="en">A module is an ontology fragment, usually identified by a unifying factor, such as a coherent theme or domain. It may include implemented patterns or be one, or be a clone/specialisation/generalisation/adaptation of an implemented pattern.</rdfs:comment>
        <rdfs:label xml:lang="en">Module</rdfs:label>
    </owl:Class>
    


    <!-- https://w3id.org/OPLa/OntologicalCollection -->

    <owl:Class rdf:about="https://w3id.org/OPLa/OntologicalCollection">
        <rdfs:comment xml:lang="en">This class represents an ontological collection, that is a collection of classes, properties, axioms, individuals formally defined.</rdfs:comment>
        <rdfs:label xml:lang="en">Ontological Collection</rdfs:label>
    </owl:Class>
    


    <!-- https://w3id.org/OPLa/OntologicalEntity -->

    <owl:Class rdf:about="https://w3id.org/OPLa/OntologicalEntity">
        <rdfs:comment xml:lang="en">An ontological entity is an axiom, class, individual or property defined in an ontological collection.</rdfs:comment>
        <rdfs:label xml:lang="en">Ontological Entity</rdfs:label>
    </owl:Class>
    


    <!-- https://w3id.org/OPLa/Ontology -->

    <owl:Class rdf:about="https://w3id.org/OPLa/Ontology">
        <rdfs:subClassOf rdf:resource="https://w3id.org/OPLa/OntologicalCollection"/>
        <rdfs:comment xml:lang="en">This class represents an ontology.</rdfs:comment>
        <rdfs:label xml:lang="en">Ontology</rdfs:label>
    </owl:Class>
    


    <!-- https://w3id.org/OPLa/OntologyDesignPattern -->

    <owl:Class rdf:about="https://w3id.org/OPLa/OntologyDesignPattern">
        <rdfs:comment xml:lang="en">An Ontology Design Pattern is a recurrent modeling solution which solves a generic modeling problem, such as how to model the roles of agents.</rdfs:comment>
        <rdfs:label xml:lang="en">Ontology Design Pattern</rdfs:label>
        <rdfs:label xml:lang="en">Pattern Template</rdfs:label>
    </owl:Class>
    


    <!-- https://w3id.org/OPLa/Property -->

    <owl:Class rdf:about="https://w3id.org/OPLa/Property">
        <rdfs:subClassOf rdf:resource="https://w3id.org/OPLa/OntologicalEntity"/>
        <rdfs:comment xml:lang="en">This class represents a property (object, datatype, annotation).</rdfs:comment>
        <rdfs:label xml:lang="en">Property</rdfs:label>
    </owl:Class>
    


    <!-- https://w3id.org/OPLa/RDFGraph -->

    <owl:Class rdf:about="https://w3id.org/OPLa/RDFGraph">
        <rdfs:comment xml:lang="en">An RDF graph is a graph of RDF triples that comply with a specific implemented pattern.</rdfs:comment>
        <rdfs:label xml:lang="en">RDF graph</rdfs:label>
    </owl:Class>
    


    <!-- 
    ///////////////////////////////////////////////////////////////////////////////////////
    //
    // Individuals
    //
    ///////////////////////////////////////////////////////////////////////////////////////
     -->

    


    <!-- https://w3id.org/OPLa/externalClass -->

    <owl:NamedIndividual rdf:about="https://w3id.org/OPLa/externalClass">
        <rdfs:label xml:lang="en">external class</rdfs:label>
    </owl:NamedIndividual>
    


    <!-- https://w3id.org/OPLa/externalIndividual -->

    <owl:NamedIndividual rdf:about="https://w3id.org/OPLa/externalIndividual">
        <rdfs:label xml:lang="en">external individual</rdfs:label>
    </owl:NamedIndividual>
    


    <!-- https://w3id.org/OPLa/externalPattern -->

    <owl:NamedIndividual rdf:about="https://w3id.org/OPLa/externalPattern">
        <rdfs:label xml:lang="en">external pattern</rdfs:label>
    </owl:NamedIndividual>
    


    <!-- https://w3id.org/OPLa/externalProperty -->

    <owl:NamedIndividual rdf:about="https://w3id.org/OPLa/externalProperty">
        <rdfs:label xml:lang="en">external property</rdfs:label>
    </owl:NamedIndividual>
</rdf:RDF>



<!-- Generated by the OWL API (version 4.5.9.2019-02-01T07:24:44Z) https://github.com/owlcs/owlapi -->

